# This file is part of dotNetRDF.
#
# dotNetRDF is free and open source software licensed under the MIT License
#
# -----------------------------------------------------------------------------
#
# Copyright (c) 2009-2013 dotNetRDF Project (dotnetrdf-develop@lists.sf.net)
#
# Permission is hereby granted, free of charge, to any person obtaining a copy
# of this software and associated documentation files (the "Software"), to deal
# in the Software without restriction, including without limitation the rights
# to use, copy, modify, merge, publish, distribute, sublicense, and/or sell
# copies of the Software, and to permit persons to whom the Software is furnished
# to do so, subject to the following conditions:
#
# The above copyright notice and this permission notice shall be included in all
# copies or substantial portions of the Software.
#
# THE SOFTWARE IS PROVIDED "AS IS", WITHOUT WARRANTY OF ANY KIND, EXPRESS OR 
# IMPLIED, INCLUDING BUT NOT LIMITED TO THE WARRANTIES OF MERCHANTABILITY, 
# FITNESS FOR A PARTICULAR PURPOSE AND NONINFRINGEMENT. IN NO EVENT SHALL THE
# AUTHORS OR COPYRIGHT HOLDERS BE LIABLE FOR ANY CLAIM, DAMAGES OR OTHER LIABILITY,
# WHETHER IN AN ACTION OF CONTRACT, TORT OR OTHERWISE, ARISING FROM, OUT OF OR IN
# CONNECTION WITH THE SOFTWARE OR THE USE OR OTHER DEALINGS IN THE SOFTWARE.

@prefix rdf: <http://www.w3.org/1999/02/22-rdf-syntax-ns#>.
@prefix rdfs: <http://www.w3.org/2000/01/rdf-schema#>.
@prefix owl: <http://www.w3.org/2002/07/owl#>.
@prefix dc: <http://purl.org/dc/elements/1.1/>.
@prefix foaf: <http://xmlns.com/foaf/0.1/>.
@prefix xsd: <http://www.w3.org/2001/XMLSchema#>.
@prefix vann: <http://purl.org/vocab/vann/>.
@prefix store: <http://www.dotnetrdf.org/StoreManager#>.

@base <http://www.dotnetrdf.org/StoreManager#>.

<http://www.dotnetrdf.org/StoreManager#> a owl:Ontology ;
   rdfs:label "dotNetRDF Store Manager Vocabulary" ;
   rdfs:comment """dotNetRDF Store Manager Vocabulary is used to in conjunction with the Configuration vocabulary to store information about managed connections.""" ;
   dc:creator [ foaf:name "Rob Vesse" ] ;
   vann:preferredNamespacePrefix "store" ;
   vann:preferredNamespaceUri <http://www.dotnetrdf.org/configuration#> .
   
store:created a rdf:Property ;
	rdfs:range xsd:dateTime ;
	rdfs:label "Created" ;
	rdfs:comment "Indicates when a connection was first created" .
	
store:lastModified a rdf:Property ;
	rdfs:range xsd:dateTime ;
	rdfs:label "Last Modified" ;
	rdfs:comment "Indicates when a connection was last modified" .
	
store:lastOpened a rdf:Property ;
	rdfs:range xsd:dateTime ;
	rdfs:label "Last Opened" ;
	rdfs:comment "Indicates when a connection was last opened" .
	
store:definitionType a rdf:Property ;
	rdfs:label "Definition Type" ;
	rdfs:comment "Used to associate serialized configuration with the IConnectionDefinition implementing type that its Configuration may be populated from." .

store:readOnly a rdf:Property ;
	rdfs:label "Read Only" ;
	rdfs:comment "Used to state that a connection should default to read only mode" ;
	rdfs:range xsd:boolean .